src/Typing.v
@@ -1,10 +1,7 @@
 From Celsius Require Export Trees.
 Require Import List.
-Import ListNotations.
 Open Scope nat_scope.
-
-
-Parameter ct: ClassTable.
+Import ListNotations.
 
 Definition fieldType C f :=
   match ct C with
@@ -16,74 +13,215 @@ Definition fieldType C f :=
     end
   end.
 
-(* Mode lattice *)
-Definition mode_leq (m1 m2 : mode) :=
-  match (m1, m2) with
-  | (hot, _ ) => true
-  | (warm, hot) => true
-  | (warm, warm) => true
-  | ( _ , cold) => true
-  | ( _ , _ ) => false end.
-Notation "m1 ⊑ m2" := (mode_leq m1 m2) (at level 100).
-
-Definition mode_max (m1 m2 : mode) : mode :=
-  match (m1 ⊑ m2) with
-  | true => m2
-  | false => m1
+Definition methodInfo C m :=
+  match ct C with
+  | None => None
+  | Some (class _ _ methods) =>
+    match methods m with
+    | None => None
+    | Some (method μ Ts retT e) => Some (μ, Ts, retT, e)
+    end
   end.
 
-Definition mode_min (m1 m2 : mode) : mode :=
-  mode_max m2 m1.
 
-Notation "m1 ⊓ m2" := (mode_min m1 m2) (at level 100).
-Notation "m1 ⊔ m2" := (mode_max m1 m2) (at level 100).
+(* Mode lattice *)
+Definition join μ1 μ2: Mode :=
+  match μ1, μ2 with
+  | hot, _ => μ2
+  | _, hot => μ1
+  | cold, _ => cold
+  | _, cold => cold
+  | _, _ => warm
+  end.
+Notation "m1 ⊔ m2" := (join m1 m2) (at level 40).
+
+Definition meet μ1 μ2 :=
+  match μ1, μ2 with
+  | hot, _ => hot
+  | _, hot => hot
+  | cold, _ => μ2
+  | _, cold => μ1
+  | _, _ => warm
+  end.
+Notation "m1 ⊓ m2" := (meet m1 m2) (at level 40).
+
+Reserved Notation "m1 ⊑ m2" (at level 40).
+Inductive S_Mode: Mode -> Mode -> Prop :=
+| s_mode_hot: forall μ, hot ⊑ μ
+| s_mode_warm: warm ⊑ warm
+| s_mode_cold: forall μ, μ ⊑ cold
+where "m1 ⊑ m2" := (S_Mode m1 m2).
+Global Hint Resolve s_mode_cold s_mode_hot s_mode_warm: typ.
+
+Lemma s_mode_refl: forall μ, μ ⊑ μ.
+Proof.
+  destruct μ; eauto with typ.
+Qed.
+Global Hint Resolve s_mode_refl: typ.
+
+Lemma s_mode_trans: forall μ1 μ2 μ3, μ1 ⊑ μ2 -> μ2 ⊑ μ3 -> μ1 ⊑ μ3.
+Proof.
+  intros.
+  inversion H; inversion H0; subst; eauto with typ; steps.
+Qed.
+Global Hint Resolve s_mode_trans: typ.
+
 
 (* Subtyping *)
+Reserved Notation "T1 <: T2" (at level 40).
+Inductive S_Typ : Tpe -> Tpe -> Prop :=
+| s_typ_mode (C: ClN) μ1 μ2: μ1 ⊑ μ2 -> (C, μ1) <: (C, μ2)
+with S_Typs : (list Tpe) -> (list Tpe) -> Prop :=
+| s_typs_nil: S_Typs nil nil
+| s_typs_cons: forall Ts1 Ts2 T1 T2,
+    S_Typs Ts1 Ts2 ->
+    T1 <: T2 ->
+    S_Typs (T1::Ts1) (T2::Ts2)
+where "T1 <: T2" := (S_Typ T1 T2).
+Global Hint Resolve s_typ_mode: typ.
 
-Reserved Notation "T1 ≲ T2" (at level 100, right associativity).
-Inductive subTyping : Tpe -> Tpe -> Prop :=
-| s_refl (T : Tpe) : (T ≲ T)
-| s_trans (T1 T2 T3 : Tpe) : (T1 ≲ T2) -> (T2 ≲ T3) -> (T1 ≲ T3)
-| s_mode (C: ClN) (μ1 μ2 : mode) (H : (μ1 ⊑ μ2) = true) : (C, μ1) ≲ (C, μ2)
-where "T1 ≲ T2" := (subTyping T1 T2).
+Lemma s_typ_refl:
+  forall T, T <: T.
+Proof.
+  destruct T; eauto with typ.
+Qed.
+Global Hint Resolve s_typ_refl: typ.
 
-Reserved Notation "'[' Γ ',' T '⊢' e ':' U ']'" (at level 60, Γ at level 60, e at level 60). (* e can have the type T in env Γ and `this` of type U *)
+Lemma s_typ_trans:
+  forall T1 T2 T3, T1 <: T2 -> T2 <: T3 -> T1 <: T3.
+Proof.
+  intros; inversion H; inversion H0; steps; eauto with typ.
+Qed.
+Global Hint Resolve s_typ_trans: typ.
 
-Definition Env := list (Var * Tpe).
+Definition P_hot (T: Tpe) :=
+  match T with
+  | (_, hot) => True
+  | _ => False
+  end.
 
-Inductive exp_typing : Env -> Tpe -> Expr -> Tpe -> Prop :=
-| t_sub :
+Definition P_hots := Forall P_hot.
+
+Lemma P_hots_In:
+  forall Ts T, P_hots Ts -> List.In T Ts -> P_hot T.
+Proof.
+  unfold P_hots; intros; eapply Forall_forall; eauto.
+Qed.
+
+(** ** Expression Typing *)
+
+Definition Env := list (Tpe).
+Reserved Notation "'[' Γ ',' T '⊢' e ':' U ']'" (at level 60, Γ at level 60, e at level 60).
+Reserved Notation "'[_' Γ ',' T '⊢' es ':' Us '_]'" (at level 60, Γ at level 60, es at level 60).
+(** e can have the type U with env Γ and `this` of type T *)
+Inductive T_Expr : Env -> Tpe -> Expr -> Tpe -> Prop :=
+| t_sub:
     forall Γ T e U U',
       [Γ, T ⊢ e : U'] ->
-      (U' ≲ U) ->
+      (U' <: U) ->
       [Γ, T ⊢ e : U]
-| t_var :
+
+| t_var:
     forall Γ T x U,
-      List.In (x, U) Γ ->
+      nth_error Γ x = Some U ->
       [Γ, T ⊢ (var x) : U]
-| t_this :
+
+| t_this:
     forall Γ T,
       [Γ, T ⊢ this : T]
-| t_selhot :
+
+| t_selhot:
     forall Γ T e f C D μ,
       [Γ, T ⊢ e : (D, hot)] ->
       (fieldType D f = Some (C, μ)) ->
       [Γ, T ⊢ (fld e f) : (C, hot)]
-| t_selwarm :
+
+| t_selwarm:
     forall Γ T e f U D,
       [Γ, T ⊢ e : (D, warm)] ->
       (fieldType D f = Some U) ->
       [Γ, T ⊢ (fld e f) : U]
 
-(*
- | t_block : forall e1 f e2 e3 C μ T1,
-    e = asgn e1 f e2 e3 ->
-    [Γ, T ⊢ e1.f : (C, μ)] ->
-    [Γ, T ⊢ e2 : (C, hot)] ->
-    [Γ, T ⊢ e3 : U] ->
-    [Γ, T ⊢ e : U] *)
+| t_new:
+    forall Γ T C args paramTs fields methods,
+      ct C = Some (class paramTs fields methods) ->
+      [_ Γ, T ⊢ args : paramTs _] ->
+      [Γ, T ⊢ (new C args) : (C, warm)]
 
-where  "'[' Γ ',' T '⊢' e ':' U ']'" := (exp_typing Γ T e U).
+| t_new_hot:
+    forall Γ T C args argsTs paramTs fields methods,
+      ct C = Some (class paramTs fields methods) ->
+      [_ Γ, T ⊢ args : argsTs _] ->
+      P_hots argsTs ->
+      S_Typs argsTs paramTs ->
+      [Γ, T ⊢ (new C args) : (C, hot)]
 
+| t_block:
+    forall Γ T U e1 f e2 e3 C μ,
+      [Γ, T ⊢ (fld e1 f) : (C, μ)] ->
+      [Γ, T ⊢ e2 : (C, hot)] ->
+      [Γ, T ⊢ e3 : U] ->
+      [Γ, T ⊢ (asgn e1 f e2 e3) : U]
 
-(* Typing *)
+| t_call:
+    forall Γ T e m args paramTs retT body μ0 μ_m C,
+      [Γ, T ⊢ e : (C, μ0)] ->
+      μ0 ⊑ μ_m ->
+      methodInfo C m = Some (μ_m, paramTs, retT, body) ->
+      [_ Γ, T ⊢ args : paramTs _] ->
+      [Γ, T ⊢ (mtd e m args) : retT]
+
+| t_call_hot:
+    forall Γ T e m args argTs paramTs D body μ0 μ_r C,
+      [Γ, T ⊢ e : (C, hot)] ->
+      (C, hot) <: (C, μ0) ->
+      methodInfo C m = Some (μ0, paramTs, (D, μ_r), body) ->
+      [_ Γ, T ⊢ args : argTs _] ->
+      P_hots argTs ->
+      S_Typs argTs paramTs ->
+      [Γ, T ⊢ (mtd e m args) : (D, hot)]
+where  "'[' Γ ',' T '⊢' e ':' U ']'" := (T_Expr Γ T e U)
+
+with T_Exprs: Env -> Tpe -> (list Expr) -> (list Tpe) -> Prop :=
+| t_exprs_nil: forall Γ T, T_Exprs Γ T [] []
+| t_exprs_cons: forall Γ T Ts es Th eh,
+    T_Exprs Γ T es Ts ->
+    [Γ, T ⊢ eh : Th] ->
+    T_Exprs Γ T (eh::es) (Th::Ts)
+where  "'[_' Γ ',' T '⊢' es ':' Us '_]'" := (T_Exprs Γ T es Us).
+
+(** ** Field typing *)
+Definition T_Field Γ T f :=
+  match f with
+  | field U e => [Γ, T ⊢ e : U]
+  end.
+Definition T_Fields Γ T := Forall (T_Field Γ T).
+
+(** ** Method typing *)
+Definition T_Method C m :=
+  match m with
+  | method μ argTs retT body => [ argTs, (C, μ) ⊢ body : retT]
+  end.
+Definition T_Methods C (methods: Mtd -> option Method) :=
+  forall id m, methods id = Some m -> T_Method C m.
+
+(** ** Class typing *)
+Definition T_Class C cl :=
+  match cl with
+  | class paramTs fields methods => T_Fields paramTs (C, cold) fields /\ T_Methods C methods
+  end.
+Fixpoint T_Classes (Ct: list Class) i :=
+  match Ct with
+  | nil => True
+  | C::Ct' => (T_Class i C) /\ (T_Classes Ct' (S i))
+  end.
+
+(** ** Program typing *)
+
+Definition T_Prog :=
+  match (ct entry) with
+  | Some (class nil nil methods) =>
+    exists e T, methods main = Some (method hot nil T e) /\
+    [nil, (entry, hot) ⊢ e : T] /\ T_Classes Ξ 0
+  | _ => False
+  end.
